c/poc/strlen_spec.v
@@ -2,7 +2,7 @@
 
 
 From Coq Require Import String List ZArith.
-From compcert Require Import Coqlib Integers Floats AST Ctypes Cop Clight Clightdefs Memory Values ClightBigstep Events.
+From compcert Require Import Coqlib Integers Floats AST Ctypes Cop Clight Clightdefs Memory Values ClightBigstep Events Maps.
 (* Local Open Scope Z_scope.*)
 
 
@@ -25,6 +25,9 @@ Fixpoint string_to_list_byte (s: string) : list byte :=
   end.
 
 Definition strlen_byte (bs : list byte) := List.length bs.
+
+Definition c_string (s : string) := (string_to_list_byte s)++(Byte.repr 0)::nil.
+Definition example := c_string "Hello".
 
 Lemma length_string_byte_equiv : forall s, String.length s = strlen_byte (string_to_list_byte s).
 Proof.
@@ -63,8 +66,9 @@ Definition is_null (v : Values.val) :=
   | _ => false
   end.
 
-Definition chunk : memory_chunk := Mint8unsigned. (* not quite sure how to deal with the memory chunks *)
+Definition chunk : memory_chunk := Mint8signed. (* not quite sure how to deal with the memory chunks *)
 Definition INTSIZE := (nat_of_Z Int.modulus).
+
 
 Definition strlen_C (m : mem) (b: block) (ofs : Z) := 
   let fix strlen_fun_C (m : mem) (b : block) (ofs : Z) (l: Z) (intrange : nat) {struct intrange} : option (Z*mem):=
@@ -114,29 +118,101 @@ Definition f_strlen := {|
 
 (* Big step semantics *)
 
-Parameter v : val.
-Parameter m : mem.
-Parameter ge : genv.
-Parameter e : env.           
+(* Require Import strlen Maps.
+Definition ge := globalenv prog. *)
 
-(* local env is a map from ident to val *)
+Parameter ge : genv. (* global environment *)
+Definition bigStepExec := ClightBigstep.exec_stmt.
+Definition t := ((E0**E0)**E0). (* trace, E0 is an empty trace *)
 
-Definition le : temp_env  := Maps.PTree.empty val.
-Definition le' := Maps.PTree.set _s v le.
-Definition le'' := Maps.PTree.set _i v le'.
+(* Find proofs on arithmetic on ptrofs type *)
+Hypothesis ptr_ofs_eq : forall ofs, ofs = (Ptrofs.unsigned
+       (Ptrofs.add (Ptrofs.repr ofs)
+                   (Ptrofs.mul (Ptrofs.repr 1) (Ptrofs.of_intu (Int.repr 0))))).
 
-(* E0 is an empty trace *)
-           
-Definition strlen_C_exec : ClightBigstep.exec_stmt ge e le' m f_strlen.(fn_body) ((E0**E0)**E0) le'' m (Out_return (Some (v,tuint))).
+(* One direction of correctness, for now the statement is wrong *)
+
+Definition strlen_C_exec_corr :
+  forall m b ofs (e : env) le z,
+    strlen_C m b ofs = Some (z,m) -> 
+    le!_s = Some (Vptr b (Ptrofs.repr ofs)) ->
+             exists le', le'!_i = Some (Vint (Int.repr z)) /\ bigStepExec ge e le m f_strlen.(fn_body) t le' m (Out_return (Some (Vint (Int.repr z),tuint))).
 Proof.
+  intros.
+  exists (Maps.PTree.set _i (Vint (Int.repr z)) le).
+  split.
+  - apply Maps.PTree.gss.
+  - repeat econstructor.
+    + rewrite PTree.gso. apply H0. eapply Pos.succ_discr. 
+    + apply PTree.gss.
+    + repeat econstructor. 
+    + simpl. rewrite <- (ptr_ofs_eq ofs). (* now need assumptions on memory, get from a lemma about strlen *) admit.
+    + simpl.  admit.
+    + simpl. admit.
+    + simpl.  admit.
+      Admitted.
+
+(* Examples of running a program: to see what assumptions need in the proof *)
+
+Parameter hi : Z.
+Definition init_mem := fst (Mem.alloc Mem.empty 0 hi).
+Definition b' := snd (Mem.alloc Mem.empty 0 hi).
+Parameter ofs' : Z.
+Hypothesis ofs_le_hi : ofs' < hi.
+
+(* Example 1 : output on empty string is correct *)
+
+Definition init_mem1 := 
+  Mem.store Mint8signed init_mem b' ofs' (Vint (Int.repr 0)).
+
+Lemma example_comp : forall m le, init_mem1 = Some m ->
+                             le!_s = Some (Vptr b' (Ptrofs.repr ofs')) ->
+                             exists le', bigStepExec ge e le m f_strlen.(fn_body) t le' m (Out_return (Some (Vint (Int.repr 0),tuint))).
+Proof.
+  intros.
+  exists (Maps.PTree.set _i (Vint (Int.repr 0)) le).
   repeat econstructor.
-  - simpl. admit. (* Addition sem_add *)
-  - simpl. (* Mem.load *) admit.
-  - simpl.  (* Comparison  sem_cmp *)  admit.
-  - simpl. (* Bool val *)  admit.
-  - admit. (* loop *)
+    + rewrite PTree.gso. apply H0. eapply Pos.succ_discr. 
+    + apply Maps.PTree.gss.
+    + econstructor.
+    + unfold init_mem1 in H. simpl. rewrite (Mem.load_store_same  Mint8signed init_mem b' _ (Vint (Int.repr 0))). constructor. rewrite <- ptr_ofs_eq. assumption.
+    + econstructor.
+    + econstructor.
+    + econstructor.
+    + apply Maps.PTree.gss.
+Qed. 
+
+(* Running on a non-empty string: some problem with the loop  *)
+
+Definition init_mem0 := fst (Mem.alloc Mem.empty 0 hi).
+Definition init_mem2 := Mem.store Mint8signed init_mem0 b' ofs' (Vint (Int.repr 1)).
+Definition init_mem3 := match init_mem2 with
+                        | None => None
+                        | Some m => Mem.store Mint8signed m b' (ofs'+1) (Vint (Int.repr 0))
+                        end.
+
+Lemma example_comp2 : forall m le,
+                          init_mem2 = Some m ->
+                          init_mem3 = Some m -> 
+                          le!_s = Some (Vptr b' (Ptrofs.repr ofs')) ->
+                          exists le', bigStepExec ge e le m f_strlen.(fn_body) t le' m (Out_return (Some (Vint (Int.repr 1),tuint))).
+Proof.
+  intros.
+  exists (Maps.PTree.set _i (Vint (Int.repr 1)) le).
+  repeat econstructor.
+    + rewrite PTree.gso. apply H1. eapply Pos.succ_discr. 
+    + apply Maps.PTree.gss.
+    + econstructor.
+    + unfold init_mem3 in H0. rewrite H in H0. simpl. rewrite <- ptr_ofs_eq.
+      unfold init_mem2 in H. rewrite <- H in H0. rewrite -> (Mem.load_store_same Mint8signed init_mem0 b' ofs' (Vint (Int.repr 1))). econstructor. assumption.
+    + econstructor.      
+    + econstructor.
+    + Print exec_stmt. admit. (* false *)
 Admitted.
 
-
-
-
+     
+(** [deref_loc ty m b ofs v] computes the value of a datum
+  of type [ty] residing in memory [m] at block [b], offset [ofs].
+  If the type [ty] indicates an access by value, the corresponding
+  memory load is performed.  If the type [ty] indicates an access by
+  reference or by copy, the pointer [Vptr b ofs] is returned. *)
